Implement 'push-button' extraction
Implement some more automated extraction that can take contracts written
for the ConCert framework and extract them to Concordium almost fully
automatically. To accomplish this we generate wrappers that convert
between the Concordium types and the ConCert types, including for the
transfer type. Calls are not yet supported.

In addition:

- Add a stack interpreter example to ConCert.Execution.Examples that
  can run in the execution layer, and extract this from RustInterp.v
  instead of the old more ad-hoc extraction.

- Implement Serializable instances for ascii/string, which were needed
  in the stack interpreter.

- Remove ForPaper.v, which is not terribly important to have in master
  anymore, since it exists in the relevant tags.

- Add a way to specify overridden masks to the dearg transform so that
  init and receive remain untouched by dearging.

- Switch the Rust counter extraction over to the version that's in
  ConCert examples since the old more ad-hoc extraction no longer works.
  In the future we may want to have the other versions of the counter in
  the ConCert framework as well so we can extract those.

- Add extraction of the Escrow contract to Concordium.

- Change the default attributes in Rust extraction as types should no
  longer require Copy.

- Add concert-std and concert-std-derive Rust packages that provide
  supporter types for our extracted contracts and also automatic
  derivation for serialization/deserialization that works with
  references and recursive types.

- Add notation <! foo %>, that from a glob-ref produces an approriate
  Coq type. For example, <! plus !> produces a kername for plus, <! nat
  !> produces an inductive and <! O !> produces an inductive * nat.

- Add and fix various more remappings when extracting Concordium.

- The ind_attrs are now properly applied to inductives instead of
  kernames.

- ##name## was allowed in remapped constants, but not in remapped type
  aliases. Fix this.

- Remove the extraction of cached cells for closures, since this was not
  fully implemented yet. We might want to implement this at some point
  to avoid excessive allocations of curried closures.

extraction/theories/Optimize.v
@@ -620,15 +620,18 @@ Record dearg_set := {
   const_masks : list (kername * bitmask);
   ind_masks : list (kername * mib_masks); }.
 
-Fixpoint analyze_env (Σ : global_env) : dearg_set :=
+Fixpoint analyze_env
+         (overridden_masks : kername -> option bitmask)
+         (Σ : global_env) : dearg_set :=
   match Σ with
   | [] => {| const_masks := []; ind_masks := [] |}
   | (kn, has_deps, decl) :: Σ =>
-    let (consts, inds) := analyze_env Σ in
+    let (consts, inds) := analyze_env overridden_masks Σ in
     let (consts, inds) :=
         match decl with
         | ConstantDecl cst =>
           let '(mask, inds) := analyze_constant cst inds in
+          let mask := option_get mask (overridden_masks kn) in
           ((kn, mask) :: consts, inds)
         | InductiveDecl mib =>
           let ctor_masks :=
@@ -662,6 +665,7 @@ Definition trim_ind_masks (im : list (kername × mib_masks)) :=
   map (on_snd trim_mib_masks) im.
 
 Definition dearg_transform
+           (overridden_masks : kername -> option bitmask)
            (* If true, trim ends of constant masks to avoid unnecessary eta expansion. *)
            (do_trim_const_masks : bool)
            (* If true, trim ends of constructor masks to avoid unnecessary eta expansion. *)
@@ -678,7 +682,8 @@ Definition dearg_transform
      else
        Ok tt);;
 
-    let (const_masks, ind_masks) := timed "Dearg analysis" (fun _ => analyze_env Σ) in
+    let (const_masks, ind_masks) := timed "Dearg analysis"
+                                          (fun _ => analyze_env overridden_masks Σ) in
 
     let const_masks := (if do_trim_const_masks then trim_const_masks else id) const_masks in
     let ind_masks := (if do_trim_ctor_masks then trim_ind_masks else id) ind_masks in
