extraction/examples/RustCounter.v
@@ -1,83 +1,32 @@
-From Coq Require Import String.
-From Coq Require Import List.
-From Coq Require Import ZArith.
-From Coq Require Import Bool.
-
-From ConCert.Extraction Require Import RustExtract.
+From ConCert.Execution Require Blockchain.
+From ConCert.Execution.Examples Require Counter.
 From ConCert.Extraction Require Import Common.
 From ConCert.Extraction Require Import ConcordiumExtract.
 From ConCert.Extraction Require Import ResultMonad.
-
-From ConCert.Extraction.Examples Require Import CounterRefinementTypes.
-From ConCert.Extraction.Examples Require Import CounterCertifiedExtraction.
+From ConCert.Extraction Require Import RustExtract.
+From Coq Require Import Bool.
+From Coq Require Import List.
+From Coq Require Import String.
+From Coq Require Import ZArith.
 From MetaCoq.Template Require Import All.
 
 Import MonadNotation.
 Import Printing.
 
-Module CR := CounterRefinementTypes.
-Module CS := CounterCertifiedExtraction.Counter.
-
 Open Scope string.
-
-Instance RustCounterConfig : RustPrintConfig :=
-  {| term_box_symbol := "()";
-     type_box_symbol := "()";
-     any_type_symbol := "()";
-     print_full_names := false |}.
-
-Definition remap_blockchain : list (kername * string) := Eval compute in
-      [ remap <%% PreludeExt.SimpleCallCtx %%> "type SimpleCallCtx<'a> = ();" ].
-
-Definition remap_address : remapped_inductive :=
-  {| re_ind_name := "AccountAddress";
-     re_ind_ctors := [];
-     re_ind_match := None |}.
-
-Definition attrs : ind_attr_map :=
-  fun kn => if eq_kername <%% CR.msg %%> kn || eq_kername <%% CS.msg %%> kn  then ["#[derive(Debug,Serialize)]"]
-         else ["#[derive(Debug, Copy, Clone)]"].
 
 Definition COUNTER_MODULE : ConcordiumMod _ _ :=
   {| concmd_contract_name := "counter";
-     concmd_init := CounterRefinementTypes.init;
-     concmd_receive := CounterRefinementTypes.counter;
-     concmd_extra := [];
-     concmd_wrap_init := init_wrapper;
-     concmd_wrap_receive := receive_wrapper_no_calls |}.
+     concmd_init := @ConCert.Execution.Examples.Counter.counter_init;
+     concmd_receive := @ConCert.Execution.Examples.Counter.counter_receive;
+     concmd_extra := []; |}.
 
-Import Blockchain.
-
-Open Scope list.
-
-Definition types_remap :=
-  ConcordiumRemap.remap_std_types
-    ++ [ (<%% @ActionBody %%>,  ConcordiumRemap.remap_Z )
-        ; (<%% nat %%>, remap_address) ].
-
-MetaCoq Run (res <- rust_extraction COUNTER_MODULE
-                           (ConcordiumRemap.build_remaps
-                              (ConcordiumRemap.remap_arith ++ remap_blockchain)
-                              [] types_remap)
-                           attrs
-                           (fun kn => eq_kername <%% bool_rec %%> kn
-                                   || eq_kername <%% bool_rect %%> kn);;
-            tmMsg res).
-
-
-Definition SIMPLE_COUNTER_MODULE : ConcordiumMod _ _ :=
-  {| concmd_contract_name := "counter";
-     concmd_init := CounterCertifiedExtraction.Counter.init;
-     concmd_receive := CounterCertifiedExtraction.Counter.counter;
-     concmd_extra := [];
-     concmd_wrap_init := init_wrapper;
-     concmd_wrap_receive := receive_wrapper_no_calls |}.
-
-MetaCoq Run (res <- rust_extraction SIMPLE_COUNTER_MODULE
-                           (ConcordiumRemap.build_remaps
-                              (ConcordiumRemap.remap_arith ++ remap_blockchain)
-                              [] types_remap)
-                           attrs
-                           (fun kn => eq_kername <%% bool_rec %%> kn
-                                   || eq_kername <%% bool_rect %%> kn);;
-            tmMsg res).
+MetaCoq Run (concordium_extraction
+               COUNTER_MODULE
+               (ConcordiumRemap.build_remaps
+                  (ConcordiumRemap.remap_arith ++ ConcordiumRemap.remap_blockchain_consts)
+                  []
+                  (ConcordiumRemap.remap_blockchain_inductives
+                     ++ ConcordiumRemap.remap_std_types))
+               (fun kn => eq_kername <%% bool_rec %%> kn
+                          || eq_kername <%% bool_rect %%> kn)).
